doc/design/DotNet/Lemmas.lean
@@ -1,0 +1,7 @@
+module
+
+public section
+
+theorem Nat.add_assoc_symm (n₁ n₂ n₃: Nat) : n₁ + (n₂ + n₃) = n₁ + n₂ + n₃ := Nat.add_assoc n₁ n₂ n₃ |> Eq.symm
+
+end --public
